Progress showing that term relation is a permutation.

crypto.v
@@ -8,7 +8,7 @@ From iris.heap_lang Require Import notation proofmode metatheory.
 From iris.heap_lang Require Import primitive_laws.
 From iris.base_logic.lib Require Import invariants.
 From iris_string_ident Require Import ltac2_string_ident.
-From crypto Require Import basic symbols.
+From crypto Require Import lib basic symbols.
 
 Section Terms.
 
@@ -90,8 +90,8 @@ Global Instance persistent_wf_nonce s l : Persistent (wf_nonce s l).
 Proof. apply _. Qed.
 
 Definition wf_key s l : iProp Σ :=
-  symbol1 lo_key_name s l ∨
-  symbol1 hi_key_name s l.
+  symbol12 lo_key_name s l ∨
+  symbol12 hi_key_name s l.
 Global Instance persistent_wf_key s l : Persistent (wf_key s l).
 Proof. apply _. Qed.
 
@@ -114,7 +114,7 @@ Definition opaque1 s t : iProp Σ :=
   | TPair _ _ => False%I
   | TNonce l => symbol1 lo_nonce_name s l
   | TKey l => False%I
-  | TEnc l t => symbol1 hi_key_name s l ∗ wf_term s t
+  | TEnc l t => symbol12 hi_key_name s l ∗ wf_term s t
   end.
 
 Global Instance persistent_opaque1 s t : Persistent (opaque1 s t).
@@ -132,8 +132,12 @@ Qed.
 
 Implicit Types TT : gsetUR (prodO valO valO).
 
+Definition term_names :=
+  [lo_nonce_name; hi_nonce_name; lo_key_name; hi_key_name].
+
 Definition opaque_inv : iProp Σ :=
-  ∃ TT, own term_name (● TT)
+  ∃ TT, ([∗ list] γ ∈ term_names, symbol_inv γ)
+        ∗ own term_name (● TT)
         ∗ ⌜perm TT⌝
         ∗ (∀ v1 v2, ⌜(v1, v2) ∈ TT⌝ -∗
            ∃ t1 t2, ⌜v1 = val_of_term t1⌝ ∗
@@ -151,7 +155,7 @@ Lemma opaque_opaque1 v1 v2 :
   opaque v1 v2 -∗
   opaque1 true (term_of_val v1) ∗ opaque1 false (term_of_val v2).
 Proof.
-iDestruct 1 as (TT) "(Hown & %Hperm & HTT)"; iIntros "#Ht1t2".
+iDestruct 1 as (TT) "(Hsymb & Hown & %Hperm & HTT)"; iIntros "#Ht1t2".
 iPoseProof (own_valid_2 with "Hown Ht1t2") as "%Hvalid".
 move: Hvalid; rewrite auth_both_valid gset_included.
 rewrite -elem_of_subseteq_singleton; case=> Ht1t2 _.
@@ -183,14 +187,33 @@ Fixpoint lo_term_aux t1 t2 : iProp Σ :=
   | TInt n1, TInt n2 => ⌜n1 = n2⌝
   | TPair t11 t12, TPair t21 t22 =>
     lo_term_aux t11 t21 ∗ lo_term_aux t12 t22
-  | TNonce l1, TNonce l2 =>
-    symbol lo_nonce_name (LR l1 l2)
+  | TNonce l1, TNonce l2 => False%I (* Nonces are covered by the opaque case
+    above *)
   | TKey l1, TKey l2 =>
     symbol lo_key_name (LR l1 l2)
   | TEnc l1 t1, TEnc l2 t2 =>
     symbol lo_key_name (LR l1 l2) ∗ lo_term_aux t1 t2
   | _, _ => False%I
   end.
+
+Definition lo_term_aux_rec t1 t2 : iProp Σ :=
+  match t1, t2 with
+  | TInt n1, TInt n2 => ⌜n1 = n2⌝
+  | TPair t11 t12, TPair t21 t22 =>
+    lo_term_aux t11 t21 ∗ lo_term_aux t12 t22
+  | TNonce l1, TNonce l2 => False%I
+  | TKey l1, TKey l2 =>
+    symbol lo_key_name (LR l1 l2)
+  | TEnc l1 t1, TEnc l2 t2 =>
+    symbol lo_key_name (LR l1 l2) ∗ lo_term_aux t1 t2
+  | _, _ => False%I
+  end.
+
+Lemma lo_term_auxE t1 t2 :
+  lo_term_aux t1 t2 =
+  (opaque (val_of_term t1) (val_of_term t2) ∨
+   lo_term_aux_rec t1 t2)%I.
+Proof. by case: t1. Qed.
 
 Global Instance persistent_lo_term_aux t1 t2 : Persistent (lo_term_aux t1 t2).
 Proof.
@@ -201,6 +224,182 @@ elim: t1 t2=> /=.
 - by move=> ?; case=> *; apply _.
 - by move=> ???; case=> *; apply _.
 Qed.
+
+Lemma flipb_lo_termE b t1 t2 :
+  flipb b lo_term_aux t1 t2 ⊣⊢
+  (flipb b opaque (val_of_term t1) (val_of_term t2) ∨
+   match t1, t2 with
+   | TInt n1, TInt n2 => ⌜n1 = n2⌝
+   | TPair t11 t12, TPair t21 t22 =>
+     flipb b lo_term_aux t11 t21 ∗ flipb b lo_term_aux t12 t22
+   | TNonce l1, TNonce l2 => False%I
+   | TKey l1, TKey l2 =>
+     symbol lo_key_name (flipb b LR l1 l2)
+   | TEnc l1 t1, TEnc l2 t2 =>
+    symbol lo_key_name (flipb b LR l1 l2) ∗ flipb b lo_term_aux t1 t2
+  | _, _ => False%I
+  end)%I.
+Proof.
+rewrite /flipb lo_term_auxE.
+case: b=> //; iSplit.
+- iDestruct 1 as "[H|H]"; eauto; iRight.
+  case: t1=> // *; case: t2=> //= *.
+  by iDestruct "H" as "->".
+- iDestruct 1 as "[H|H]"; eauto; iRight.
+  case: t1=> // *; case: t2=> //= *.
+  by iDestruct "H" as "->".
+Qed.
+
+Lemma flipb_opaque_perm b v1 v21 v22 :
+  opaque_inv -∗
+  flipb b opaque v1 v21 -∗
+  flipb b opaque v1 v22 -∗
+  ⌜v21 = v22⌝.
+Proof.
+iDestruct 1 as (TT) "(_ & Hown & %Hperm & HTT)".
+rewrite /flipb /opaque; case: b=> /=.
+- iIntros "Hown1 Hown2".
+  iPoseProof (own_valid_2 with "Hown Hown1") as "%Hval1".
+  iPoseProof (own_valid_2 with "Hown Hown2") as "%Hval2".
+  move: Hval1; rewrite auth_both_valid gset_included; case=> Hval1 _.
+  move: Hval2; rewrite auth_both_valid gset_included; case=> Hval2 _.
+  move: Hval1 Hval2; rewrite -!elem_of_subseteq_singleton=> Hval1 Hval2.
+  iPureIntro; by apply (Hperm _ _ Hval1 Hval2).
+- iIntros "Hown1 Hown2".
+  iPoseProof (own_valid_2 with "Hown Hown1") as "%Hval1".
+  iPoseProof (own_valid_2 with "Hown Hown2") as "%Hval2".
+  move: Hval1; rewrite auth_both_valid gset_included; case=> Hval1 _.
+  move: Hval2; rewrite auth_both_valid gset_included; case=> Hval2 _.
+  move: Hval1 Hval2; rewrite -!elem_of_subseteq_singleton=> Hval1 Hval2.
+  iPureIntro; by apply (Hperm _ _ Hval1 Hval2).
+Qed.
+
+Lemma flipb_opaque_opaque1 b v1 v2 :
+  opaque_inv -∗
+  flipb b opaque v1 v2 -∗
+  opaque1 b (term_of_val v1).
+Proof.
+rewrite /flipb; case: b=> /=.
+- exact: opaque_opaque1L.
+- exact: opaque_opaque1R.
+Qed.
+
+Lemma flipb_lo_term_perm b t1 t21 t22 :
+  opaque_inv -∗
+  flipb b lo_term_aux t1 t21 -∗
+  flipb b lo_term_aux t1 t22 -∗
+  ⌜t21 = t22⌝.
+Proof.
+elim: t1 t21 t22.
+- move=> n1 t21 t22; iIntros "Hinv #H1 #H2".
+  rewrite !flipb_lo_termE.
+  iDestruct "H1" as "[H1|H1]".
+    by iDestruct (flipb_opaque_opaque1 with "Hinv H1") as "[]".
+  iDestruct "H2" as "[H2|H2]".
+    by iDestruct (flipb_opaque_opaque1 with "Hinv H2") as "[]".
+  case: t21=> // ?; iDestruct "H1" as "<-".
+  by case: t22=> // ?; iDestruct "H2" as "<-".
+- move=> t11 IH1 t12 IH2 t21 t22; iIntros "Hinv #H1 #H2".
+  rewrite !flipb_lo_termE.
+  iDestruct "H1" as "[H1|H1]".
+    by iDestruct (flipb_opaque_opaque1 with "Hinv H1") as "[]".
+  iDestruct "H2" as "[H2|H2]".
+    by iDestruct (flipb_opaque_opaque1 with "Hinv H2") as "[]".
+  case: t21=> //= t211 t212; iDestruct "H1" as "[H11 H12]".
+  case: t22=> //= t221 t222; iDestruct "H2" as "[H21 H22]".
+  iDestruct (IH1 with "Hinv H11 H21") as "%".
+  iDestruct (IH2 with "Hinv H12 H22") as "%".
+  iPureIntro; congruence.
+- move=> l t21 t22; iIntros "Hinv #H1 #H2".
+  rewrite !flipb_lo_termE /=.
+  iDestruct "H1" as "[H1|H1]"; last by case: t21.
+  iDestruct "H2" as "[H2|H2]"; last by case: t22.
+  iPoseProof (flipb_opaque_perm with "Hinv H1 H2") as "%E".
+  by iPureIntro; apply: val_of_term_inj.
+- move=> l t21 t22; iIntros "Hinv #H1 #H2".
+  rewrite !flipb_lo_termE /=.
+  iDestruct "H1" as "[H1|H1]".
+    by iDestruct (flipb_opaque_opaque1 with "Hinv H1") as "[]".
+  iDestruct "H2" as "[H2|H2]".
+    by iDestruct (flipb_opaque_opaque1 with "Hinv H2") as "[]".
+  case: t21=> //= l21; case: t22=> //= l22.
+  iDestruct "Hinv" as (?) "[Hsymb _]".
+  rewrite !(big_sepL_singleton, big_sepL_cons).
+  iDestruct "Hsymb" as "(_ & _ & Hlo_key & _)".
+  iPoseProof (flipb_symbol_perm with "Hlo_key H1 H2") as "%E".
+  by rewrite E.
+- move=> l1 t1 IH t21 t22; iIntros "Hinv #H1 #H2".
+  rewrite !flipb_lo_termE.
+  iDestruct "H1" as "[H1|H1]"; iDestruct "H2" as "[H2|H2]".
+  + iPoseProof (flipb_opaque_perm with "Hinv H1 H2") as "%E".
+    iPureIntro; exact: val_of_term_inj.
+  + case: t22=> //= l22 t22; iDestruct "H2" as "[H2 _]".
+    iPoseProof (flipb_opaque_opaque1 with "Hinv H1") as "#H1' /=".
+    iDestruct "H1'" as "[H1' _]".
+    (* Need to ensure that different key types are disjoint *)
+    admit.
+  + case: t21=> //= l21 t21; iDestruct "H1" as "[H1 _]".
+    iPoseProof (flipb_opaque_opaque1 with "Hinv H2") as "#H2' /=".
+    iDestruct "H2'" as "[H2' _]".
+    (* Need to ensure that different key types are disjoint *)
+    admit.
+  + case: t21 t22=> //= l21 t21 [] //= l22 t22.
+    iDestruct "H1" as "[Hl21 Ht21]".
+    iDestruct "H2" as "[Hl22 Ht22]".
+    iPoseProof (IH with "Hinv Ht21 Ht22") as "%Et".
+    iDestruct "Hinv" as (TT) "[Hsymb _]".
+    rewrite !(big_sepL_singleton, big_sepL_cons).
+    iDestruct "Hsymb" as "(? & ? & Hlo_key & ?)".
+    iPoseProof (flipb_symbol_perm with "Hlo_key Hl21 Hl22") as "%El".
+    iPureIntro; congruence.
+Admitted.
+
+Lemma lo_term_perm t11 t12 t21 t22 :
+  opaque_inv -∗
+  lo_term_aux t11 t12 -∗
+  lo_term_aux t21 t22 -∗
+  ⌜t11 = t21 ↔ t12 = t22⌝.
+Proof.
+elim: t11 t12 t21 t22.
+- move=> n1 t12 t21 t22; iIntros "Hinv #H1 #H2".
+  iDestruct "H1" as "[H1|H1]".
+    by iDestruct (opaque_opaque1L with "Hinv H1") as "[]".
+  case: t12=> //= ?; iDestruct "H1" as "<-".
+  rewrite /iff; iSplit; iIntros (e).
+  + rewrite -{t21}e; iDestruct "H2" as "[H2|H2]".
+      by iDestruct (opaque_opaque1L with "Hinv H2") as "[]".
+    by case: t22=> //= n2; iDestruct "H2" as "<-".
+  + rewrite lo_term_auxE -{t22}e; iDestruct "H2" as "[H2|H2]".
+      by iDestruct (opaque_opaque1R with "Hinv H2") as "[]".
+    by case: t21=> //= n2; iDestruct "H2" as "<-".
+- move=> t111 IH1 t112 IH2 t12 t21 t22; iIntros "Hinv #H1 #H2 /=".
+  iDestruct "H1" as "[H1|H1]".
+    by iDestruct (opaque_opaque1L with "Hinv H1") as "[]".
+  case: t12=> //= t121 t122.
+  iDestruct "H1" as "[H11 H12]".
+  rewrite /iff; iSplit; iIntros (e).
+  + rewrite -{t21}e /=; iDestruct "H2" as "[H2|H2]".
+      by iDestruct (opaque_opaque1L with "Hinv H2") as "[]".
+    case: t22=> //= t221 t222.
+    iDestruct "H2" as "[H21 H22]".
+    iPoseProof (IH1 with "Hinv H11 H21") as "%e1".
+    iPoseProof (IH2 with "Hinv H12 H22") as "%e2".
+    iPureIntro.
+
+
+[n2| | | |] //=.
+  + move=> t21 t22.
+    iDestruct "H1" as "[H1|<-]".
+      by iPoseProof (opaque_opaque1R with "Hinv H1") as "#? /=".
+    rewrite /iff; iSplit; iIntros (e).
+    * rewrite -{}e.
+      iDestruct "H2" as "[H2|H2]".
+
+  match goal with
+  | |- context[environments.Esnoc _ (INamed ?H) (_ ∨ False)%I] =>
+    idtac H
+  end.
+
 
 Definition lo_term v1 v2 : iProp Σ :=
   ∃ t1 t2, ⌜v1 = val_of_term t1⌝ ∗
