lib.v
@@ -1,0 +1,7 @@
+From stdpp Require Import base countable gmap.
+
+Definition perm `{!EqDecision T, !Countable T} (X : gset (T * T)) :=
+  forall p1 p2, p1 ∈ X → p2 ∈ X → (p1.1 = p2.1 ↔ p1.2 = p2.2).
+
+Definition flipb {T S} (b : bool) (f : T → T → S) x y :=
+  f (if b then x else y) (if b then y else x).
